

$$\sum_{n=0}^{\infty} \frac{a^n n!}{n^n}$$

$$\lim_{n \rightarrow \infty} s_n = ?$$

$$\lim_{n \rightarrow \infty} \frac{x_{n+1}}{x_n} = \lim_{n \rightarrow \infty} \frac{\frac{a^{n+1}(n+1)!}{(n+1)^{n+1}}}{\frac{a^n n!}{n^n}} = \lim_{n \rightarrow \infty} \frac{a(n+1)n^n}{(n+1)^{n+1}} = \lim_{n \rightarrow \infty} \frac{an^n}{(n+1)^n} = \lim_{n \rightarrow \infty} \frac{an^n}{n^n(1+1/n)^n} = \lim_{n \rightarrow \infty} \frac{a}{(1+1/n)^n} = \frac{a}{e}$$

Discuție:

$$l < 1 \Leftrightarrow \frac{a}{e} < 1 \Rightarrow \sum_{n=0}^{\infty} x_n \text{ este convergentă}$$

$$l > 1 \Leftrightarrow \frac{a}{e} > 1 \Rightarrow \sum_{n=0}^{\infty} x_n \text{ este divergentă}$$

$$l = 1 \Leftrightarrow \frac{a}{e} = 1 \Rightarrow \text{nu putem determina cu criteriul raportului}$$

$$\text{pt. } \frac{a}{e} = 1 \Leftrightarrow a = e, x_n = \frac{e^n n!}{n^n}$$

$$\lim_{n \rightarrow \infty} n \left( \frac{x_n}{x_{n+1}} - 1 \right) = \lim_{n \rightarrow \infty} n \left( \frac{(1+1/n)^n}{e} - 1 \right) = \underbrace{\lim_{n \rightarrow \infty} \frac{\frac{(1+1/n)^n}{e} - 1}{\frac{1}{n}}}_{\text{limită de serii}} = \underbrace{\lim_{x \rightarrow 0} \frac{\frac{(1+x)^{1/x}}{e} - 1}{x}}_{1/n=x \text{ limită de funcție}} \stackrel{\frac{0}{0}}{\underset{\text{L'H}}{=}} \lim_{x \rightarrow 0} \frac{\frac{1}{e} \left( (1+x)^{1/x} \right)'}{x'} =$$

$$\begin{aligned} \left( (1+x)^{1/x} \right)' &= \left( \left( e^{\frac{\ln(1+x)}{x}} \right)^{1/x} \right)' = \left( e^{\frac{\ln(1+x)}{x}} \right)' = e^{\frac{\ln(1+x)}{x}} \left( \frac{\ln(1+x)}{x} \right)' = (1+x)^{1/x} \frac{\frac{1}{1+x}x - \ln 1 + x}{x^2} \\ &= \frac{1}{e} \lim_{x \rightarrow 0} \underbrace{(1+x)^{1/x}}_e \frac{\frac{x}{1+x} - \ln 1 + x}{x^2} = \lim_{x \rightarrow 0} \frac{x - (1+x)\ln(1+x)}{x^2 \underbrace{(x+1)}_1} = \lim_{x \rightarrow 0} \frac{x - (1+x)\ln(1+x)}{x^2} \stackrel{\frac{0}{0}}{\underset{\text{L'H}}{=}} \lim_{x \rightarrow 0} \frac{1 - (\ln(1+x) + 1)}{2x} \stackrel{\frac{0}{0}}{\underset{\text{L'H}}{=}} \end{aligned}$$

$$= -\lim_{x \rightarrow 0} \frac{\frac{1}{1+x}}{2} = -\frac{1}{2} \Leftrightarrow \lim_{n \rightarrow 0} n \left( \frac{x_n}{x_{n+1}} - 1 \right) = -\frac{1}{2} < 0 \Rightarrow \sum_{n=0}^{\infty} x_n \text{ este divergentă}$$

Deci:

$$\text{pt. } a < e, s_n \text{ este convergentă}$$

$$\text{pt. } a \geq e, s_n \text{ este divergentă}$$

$$f_n : \mathbb{R} \rightarrow \mathbb{R}, f_n(x) = \frac{2nx}{n^2 + x^3}, \forall n \in \mathbb{N}$$

$$\lim_{n \rightarrow \infty} f_n = \lim_{n \rightarrow \infty} \frac{2nx}{n^2 + x^3} = 0$$

$$f : \mathbb{R} \rightarrow \mathbb{R}, f(x) = 0, \forall x \in \mathbb{R}$$

$$f_n \xrightarrow[\mathbb{R}]s f$$

$$\lim_{n \rightarrow \infty} \sup_{x \in \mathbb{R}} |f_n(x) - f(x)| = \lim_{n \rightarrow \infty} \sup_{x \in \mathbb{R}} \left| \frac{2nx}{n^2 + x^3} - 0 \right| = \lim_{n \rightarrow \infty} \sup_{x \in \mathbb{R}} \underbrace{\left| \frac{2nx}{n^2 + x^3} \right|}_{g(x)}$$

$$g'(x) = \left( \frac{2nx}{n^2 + x^3} \right)' = \frac{(2nx)'(n^2 + x^3) - (2nx)(n^2 + x^3)'}{(n^2 + x^3)^2} = \frac{2n^3 - 4nx^3}{(n^2 + x^3)^2} = 0 \Rightarrow 2n^3 - 4nx^3 = 0 \Rightarrow 4nx^3 = 2n^3 \Rightarrow$$

$$\Rightarrow x^3 = \frac{n^2}{2} \Rightarrow x = \sqrt[3]{\frac{n^2}{2}}$$

$x$	$-\infty$	$\sqrt[3]{\frac{n^2}{2}}$	$\infty$
$g'(x)$	$+$	$0$	$-$
$g(x)$	$0$	$\nearrow \frac{2n \sqrt[3]{\frac{n^2}{2}}}{n^2 + \frac{n^2}{2}} \searrow 0$	$0$

$$\lim_{n \rightarrow \infty} \sup_{x \in \mathbb{R}} |f_n(x) - f(x)| = \lim_{n \rightarrow \infty} \frac{2n \sqrt[3]{\frac{n^2}{2}}}{n^2 + \frac{n^2}{2}} = \lim_{n \rightarrow \infty} \frac{2n \sqrt[3]{\frac{n^2}{2}}}{n^2 + \frac{n^2}{2}} = \lim_{n \rightarrow \infty} \frac{4n^{\frac{2}{3}+1}}{\sqrt[3]{2}(2n^2 + n^2)} = \lim_{n \rightarrow \infty} \frac{4n^{\frac{5}{3}}}{3\sqrt[3]{2}n^2} = \lim_{n \rightarrow \infty} \frac{4}{3\sqrt[3]{2}n} = 0 \Rightarrow f_n \xrightarrow[(2,5)]u f$$

$$f_n : [0, \infty) \rightarrow \mathbb{R}, f_n(x) = x^4 e^{-nx+5}, \forall n \in \mathbb{N}$$

$$\lim_{n \rightarrow \infty} f_n = \lim_{n \rightarrow \infty} x^4 e^{-nx+5} = 0$$

$$f : [0, \infty) \rightarrow \mathbb{R}, f(x) = 0, \forall x \in \mathbb{R}$$

$$f_n \xrightarrow[\mathbb{R}]s f$$

$$\lim_{n \rightarrow \infty} \sup_{x \in \mathbb{R}} |f_n(x) - f(x)| = \lim_{n \rightarrow \infty} \sup_{x \in \mathbb{R}} |x^4 e^{-nx+5} - 0| = \lim_{n \rightarrow \infty} \sup_{x \in \mathbb{R}} \underbrace{|x^4 e^{-nx+5}|}_{g(x)}$$

$$g'(x) = (x^4 e^{-nx+5})' = 4x^3 e^{-nx+5} + x^4 e^{-nx+5}(-n) = x^3 e^{-nx+5}(4 - nx) = 0 \Rightarrow \begin{cases} x^3 = 0 \Leftrightarrow x = 0 \\ 4 - nx = 0 \Leftrightarrow nx = 4 \Leftrightarrow x = \frac{4}{n} \in [0, \infty) \end{cases}$$

$x$	$0$	$\frac{4}{n}$	$\infty$
$g'(x)$	$0$	$+$	$-$
$g(x)$	$0$	$\nearrow \left(\frac{4}{n}\right)^4 e \searrow 0$	$0$

$$\lim_{n \rightarrow \infty} \sup_{x \in \mathbb{R}} |f_n(x) - f(x)| = \lim_{n \rightarrow \infty} \left(\frac{4}{n}\right)^4 e = 0 \Rightarrow f_n \xrightarrow[(2,5)]u f$$